Updated muxer specs

new/proof/github_com/goose_lang/goose/testdata/examples/channel.v
@@ -935,26 +935,23 @@ Instance mapper_service_prot_unfold Φpre Φpost :
     (mapper_service_prot_aux Φpre Φpost (mapper_service_prot Φpre Φpost)).
 Proof. apply proto_unfold_eq, (fixpoint_unfold _). Qed.
 
-Definition is_mapper_stream (stream req_ch res_ch: loc) (f: func.t)
-    (f_log: go_string → go_string) : iProp Σ :=
-  "req" ∷ stream ↦s[chan_spec_raw_examples.stream :: "req"] req_ch ∗
-  "res" ∷ stream ↦s[chan_spec_raw_examples.stream :: "res"] res_ch ∗
-  "f"   ∷ stream ↦s[chan_spec_raw_examples.stream :: "f"] f ∗
-  "Hf_spec" ∷ (∀ (s: go_string),
-      WP #f #s {{ λ v, ∃ (s': go_string), ⌜v = #s'⌝ ∗ ⌜s' = f_log s⌝ }}).
-
+Definition is_mapper_stream stream
+  (Φpre : go_string → iProp Σ) (Φpost : go_string → go_string → iProp Σ) : iProp Σ :=
+  ∃ req_ch res_ch f,
+  ⌜stream = {| stream.req' := req_ch; stream.res' := res_ch; stream.f' := f |}⌝ ∗
+  "Hf_spec" ∷ □ (∀ (s: go_string),
+      Φpre s → WP #f #s {{ λ v, ∃ (s': go_string), ⌜v = #s'⌝ ∗ Φpost s s' }}) ∗
+    # (res_ch, req_ch) ↣ iProto_dual (mapper_service_prot Φpre Φpost).
 
 Lemma wp_mkStream (f: func.t) Φpre Φpost :
   {{{ is_pkg_init chan_spec_raw_examples ∗
-      is_pkg_init channel ∗
-      (∀ (s: go_string),
-         Φpre s -∗ WP #f #s {{ λ v, ∃ (s': go_string), ⌜v = #s'⌝ ∗ Φpost s s' }})
-  }}}
+        "#Hf_spec" ∷ □ (∀ (strng: go_string),
+          Φpre strng -∗ WP #f #strng
+          {{ λ v, ∃ (s': go_string), ⌜v = #s'⌝ ∗ Φpost strng s' }}) }}}
     @! chan_spec_raw_examples.mkStream #f
-  {{{ (req_ch res_ch: loc) stream, RET stream;
-      # (req_ch, res_ch) ↣ mapper_service_prot Φpre Φpost ∗
-      # (res_ch, req_ch) ↣ iProto_dual (mapper_service_prot Φpre Φpost)
-  }}}.
+  {{{ stream, RET #stream;
+      is_mapper_stream stream Φpre Φpost ∗
+    # (stream.(stream.req'), stream.(stream.res')) ↣ mapper_service_prot Φpre Φpost }}}.
 Proof.
   wp_start. wp_auto.
       wp_apply (chan.wp_make (V:=go_string)); first done.
@@ -964,30 +961,30 @@ Proof.
   iIntros (ch1). iIntros (γ1). iIntros "(#HisChan1 & Hownchan1)".
   wp_apply wp_fupd.
 
-  iMod (dsp_session_init _ _ _ _ _ _ _ _ _
-          (mapper_service_prot Φpre Φpost) with "HisChan HisChan1 Hownchan
- Hownchan1")
+  iMod (dsp_session_init _ ch1 ch _ _ _ _ _ _
+          (mapper_service_prot Φpre Φpost) with "HisChan1 HisChan Hownchan1
+ Hownchan")
                        as "[Hpl Hpr]";
     [by eauto|by eauto|..].
   iModIntro. wp_auto.
   iApply "HΦ".
-  iFrame "Hpl Hpr".
+  rewrite /is_mapper_stream.
+  iSplitR "Hpl".
+  { iExists _, _, _. iSplit; [done|].
+    iDestruct "Hpre" as "#Hpre". iFrame "Hpr".
+    iIntros "!>" (s) "HΦ". by iApply "Hpre". }
+  iFrame "Hpl".
 Qed.
 
 Lemma wp_MapServer (my_stream: stream.t) Φpre Φpost :
-  {{{ is_pkg_init chan_spec_raw_examples ∗
-      "#Hf_spec" ∷ □ (∀ (strng: go_string),
-          Φpre strng -∗
-          WP #(my_stream.(stream.f')) #strng
-          {{ λ v, ∃ (s': go_string), ⌜v = #s'⌝ ∗ Φpost strng s' }}) ∗
-      "Hprot" ∷ # (my_stream.(stream.res'), my_stream.(stream.req')) ↣
-                   iProto_dual (mapper_service_prot Φpre Φpost)}}}
+  {{{ is_pkg_init chan_spec_raw_examples ∗ is_mapper_stream my_stream Φpre Φpost }}}
     @! chan_spec_raw_examples.MapServer #my_stream
   {{{ RET #(); True }}}.
 Proof using chanGhostStateG1 dspG0 ext ffi ffi_interp0 ffi_semantics0 globalsGS0 go_ctx hG Σ.  wp_start.
   iNamed "Hpre".
   rewrite /chan.for_range.
   wp_auto.
+  iDestruct "Hpre" as (Heq) "[#Hf_spec Hprot]".
   iAssert (∃ (in_val: go_string),
     "in" ∷ in_ptr ↦ in_val ∗
     "s" ∷ s_ptr ↦ my_stream ∗
@@ -995,7 +992,7 @@ Proof using chanGhostStateG1 dspG0 ext ffi ffi_interp0 ffi_semantics0 globalsGS0
     "Hprot" ∷ # (my_stream.(stream.res'), my_stream.(stream.req')) ↣
                  iProto_dual (mapper_service_prot Φpre Φpost)
   )%I with "[in s Hf_spec Hprot]" as "IH".
-  { iExists _. iFrame. }
+  { iExists _. iFrame. subst. iFrame. }
 
   wp_for.
   iNamed "IH".
@@ -1006,7 +1003,7 @@ Proof using chanGhostStateG1 dspG0 ext ffi ffi_interp0 ffi_semantics0 globalsGS0
 
   wp_bind (#my_stream.(stream.f') #req_val)%E.
   iApply (wp_wand with "[Hf_spec Hreq]").
-  { iSpecialize ("Hf_spec" $! req_val). iApply ("Hf_spec" with "Hreq"). }
+  { iSpecialize ("Hf_spec" $! req_val). subst. iApply ("Hf_spec" with "Hreq"). }
   iIntros (v) "Hv".
   iDestruct "Hv" as (s') "[%Heq_v Heq_log]".
   subst.
@@ -1021,12 +1018,7 @@ Qed.
 Lemma wp_Muxer (c: loc) γmpmc (n_prod n_cons: nat) :
   {{{ is_pkg_init chan_spec_raw_examples ∗
       "#Hismpmc" ∷ is_mpmc γmpmc c n_prod n_cons
-        (λ s, ∃ Φpre Φpost,
-            □ (∀ (strng: go_string),
-                Φpre strng -∗ WP #(s.(stream.f')) #strng
-                {{ λ v, ∃ (s': go_string), ⌜v = #s'⌝ ∗ Φpost strng s' }}) ∗
-            # (s.(stream.res'), s.(stream.req')) ↣
-              iProto_dual (mapper_service_prot Φpre Φpost))
+        (λ s, ∃ Φpre Φpost, is_mapper_stream s Φpre Φpost)
         (λ _, True) ∗
       "Hcons" ∷ mpmc_consumer γmpmc (∅ : gmultiset stream.t) }}}
     @! chan_spec_raw_examples.Muxer #c
